Finished removing tyvars

02Typed/Typechecking.thy
@@ -48,6 +48,12 @@ primrec liquify :: "ty expr\<^sub>s \<Rightarrow> uterm expr\<^sub>s" where
 | "liquify (Lam\<^sub>s x t e) = Lam\<^sub>s x (untypeify t) (liquify e)"
 | "liquify (App\<^sub>s e\<^sub>1 e\<^sub>2) = App\<^sub>s (liquify e\<^sub>1) (liquify e\<^sub>2)"
 
+primrec partial_solidify :: "var set \<Rightarrow> uterm expr\<^sub>s \<Rightarrow> uterm expr\<^sub>s" where
+  "partial_solidify vs (Var\<^sub>s x) = Var\<^sub>s x"
+| "partial_solidify vs (Const\<^sub>s k) = Const\<^sub>s k"
+| "partial_solidify vs (Lam\<^sub>s x t e) = Lam\<^sub>s x (partial_typeify vs t) (partial_solidify vs e)"
+| "partial_solidify vs (App\<^sub>s e\<^sub>1 e\<^sub>2) = App\<^sub>s (partial_solidify vs e\<^sub>1) (partial_solidify vs e\<^sub>2)"
+
 fun typecheck :: "'a expr\<^sub>s \<rightharpoonup> ty expr\<^sub>s \<times> ty" where
   "typecheck e = (
     let (e', t, vs, con) = typecheck' Map.empty {} e
@@ -96,10 +102,16 @@ lemma [simp]: "valid_ty_hexpr e \<Longrightarrow> htvars e = {} \<Longrightarrow
 lemma [simp]: "erase (solidify (hsubst sub e)) = erase (solidify e)"
   by (induction e) simp_all
 
+lemma [simp]: "htvars t = {} \<Longrightarrow> partial_solidify vs t = t"
+  by (induction t) simp_all
+
+lemma [simp]: "x \<notin> htvars t \<Longrightarrow> partial_solidify (insert x vs) t = partial_solidify vs t"
+  by (induction t) simp_all
+
 lemma [simp]: "valid_ty_subst sub \<Longrightarrow> valid_ty_hexpr e \<Longrightarrow> valid_ty_hexpr (hsubst sub e)"
   by (induction e) simp_all
 
-lemma [simp]: "htvars (hsubst sub e) \<subseteq> htvars e - dom sub \<union> subst_vars sub"
+lemma htvars_hsubst [simp]: "htvars (hsubst sub e) \<subseteq> htvars e - dom sub \<union> subst_vars sub"
 proof (induction e)
   case (Lam\<^sub>s x t e)
   moreover have "uvars (subst sub t) \<subseteq> uvars t - dom sub \<union> subst_vars sub" by simp
@@ -236,13 +248,37 @@ proof -
   ultimately show "x \<notin> uvars t'" by auto
 qed
 
+lemma [simp]: "typecheck' \<Gamma> vs e = (e', t', vs', con) \<Longrightarrow> finite vs \<Longrightarrow> 
+  constr_vars con \<subseteq> vs' - vs \<union> subst_vars \<Gamma>"
+proof (induction rule: typecheck_induct)
+  case (Lam\<^sub>s \<Gamma> vs vs' con x u e\<^sub>1 e\<^sub>1' t' v)
+  moreover hence "insert v vs \<subseteq> vs'" by (metis vars_expand)
+  ultimately show ?case by auto
+next
+  case (App\<^sub>s \<Gamma> vs vs' e\<^sub>1 e\<^sub>2 v e\<^sub>1' t\<^sub>1 vs'' con\<^sub>1 e\<^sub>2' t\<^sub>2 con\<^sub>2)
+  moreover hence V1: "insert v vs \<subseteq> vs''" by (metis vars_expand)
+  moreover from App\<^sub>s have V2: "vs'' \<subseteq> vs'" by (metis vars_expand)
+  ultimately have V: "v \<in> vs' \<and> v \<notin> vs" by auto
+  from App\<^sub>s have "constr_vars con\<^sub>1 \<subseteq> vs'' - insert v vs \<union> subst_vars \<Gamma>" by simp
+  with V2 have C1: "constr_vars con\<^sub>1 \<subseteq> vs' - vs \<union> subst_vars \<Gamma>" by auto
+  from App\<^sub>s have "constr_vars con\<^sub>2 \<subseteq> vs' - vs'' \<union> subst_vars \<Gamma>" by simp
+  with V1 have C2: "constr_vars con\<^sub>2 \<subseteq> vs' - vs \<union> subst_vars \<Gamma>" by auto
+  from App\<^sub>s have "uvars t\<^sub>1 \<subseteq> vs'' - insert v vs \<union> subst_vars \<Gamma>" by simp
+  with V2 have T1: "uvars t\<^sub>1 \<subseteq> vs' - vs \<union> subst_vars \<Gamma>" by auto
+  from App\<^sub>s have "uvars t\<^sub>2 \<subseteq> vs' - vs'' \<union> subst_vars \<Gamma>" by simp
+  with V1 have "uvars t\<^sub>2 \<subseteq> vs' - vs \<union> subst_vars \<Gamma>" by auto
+  with V C1 C2 T1 show ?case by simp
+qed simp_all
+
 lemma [simp]: "typecheck' \<Gamma> vs e = (e', t', vs', con) \<Longrightarrow> x \<in> vs \<Longrightarrow> finite vs \<Longrightarrow>
   x \<notin> subst_vars \<Gamma> \<Longrightarrow> x \<notin> constr_vars con"
-proof (induction rule: typecheck_induct)
-  case (App\<^sub>s \<Gamma> vs vs' e\<^sub>1 e\<^sub>2 v e\<^sub>1' t\<^sub>1 vs'' con\<^sub>1 e\<^sub>2' t\<^sub>2 con\<^sub>2)
-  moreover hence "x \<in> vs''" using vars_expand by fastforce
-  ultimately show ?case by auto
-qed fastforce+
+proof -
+  assume "typecheck' \<Gamma> vs e = (e', t', vs', con)"
+     and "finite vs"
+  hence "constr_vars con \<subseteq> vs' - vs \<union> subst_vars \<Gamma>" by simp
+  moreover assume "x \<in> vs" and "x \<notin> subst_vars \<Gamma>" 
+  ultimately show "x \<notin> constr_vars con" by auto
+qed
 
 lemma [simp]: "typecheck' (\<Gamma>(x \<mapsto> Var y)) vs e = (e', tt, vs', con) \<Longrightarrow> y \<in> vs \<Longrightarrow>
   subst_vars \<Gamma> \<subseteq> vs - {y} \<Longrightarrow> uvars t' \<subseteq> vs - {y} \<Longrightarrow> finite vs \<Longrightarrow> typecheck' (\<Gamma>(x \<mapsto> t')) vs e = 
@@ -326,8 +362,9 @@ qed auto
 
 lemma typecheck_fails' [simp]: "map_option typeify \<circ> \<Gamma> \<turnstile>\<^sub>n e\<^sub>t : t \<Longrightarrow> finite vs \<Longrightarrow> 
   subst_vars \<Gamma> \<subseteq> vs \<Longrightarrow> valid_ty_subst \<Gamma> \<Longrightarrow> typecheck' \<Gamma> vs (erase e\<^sub>t) = (e', tt, vs', con) \<Longrightarrow> 
-  \<exists>s. solidify (hsubst s e') = e\<^sub>t \<and> typeify (subst s tt) = t \<and> dom s = vs' - vs \<and> 
-  subst_vars s \<subseteq> subst_vars \<Gamma> \<and> s unifies\<^sub>\<kappa> con \<and> valid_ty_subst s \<and> idempotent s"
+  \<exists>s. partial_solidify vs (hsubst s e') = liquify e\<^sub>t \<and> 
+  partial_typeify vs (subst s tt) = untypeify t \<and> dom s = vs' - vs \<and> 
+  subst_vars s = {} \<and> s unifies\<^sub>\<kappa> partial_typeify_constr vs con \<and> valid_ty_subst s \<and> idempotent s"
 proof (induction "map_option typeify \<circ> \<Gamma>" e\<^sub>t t arbitrary: \<Gamma> vs e' tt vs' con rule: typecheckn.induct)
   case (tcn_lam x t\<^sub>1 e t\<^sub>2)
   let ?v = "fresh vs"
@@ -344,31 +381,51 @@ proof (induction "map_option typeify \<circ> \<Gamma>" e\<^sub>t t arbitrary: \<
      constr_subst ?v (untypeify t\<^sub>1) con')" by simp
   from tcn_lam have "finite (insert ?v vs)" by simp
   with tcn_lam X Y Z TC obtain s where S: "
-    solidify (hsubst s (hsubst [?v \<mapsto> untypeify t\<^sub>1] e'')) = e \<and> 
-    typeify (subst s (subst [?v \<mapsto> untypeify t\<^sub>1] t')) = t\<^sub>2 \<and>
-    s unifies\<^sub>\<kappa> constr_subst ?v (untypeify t\<^sub>1) con' \<and> dom s = vs'' - insert ?v vs \<and> 
-    subst_vars s \<subseteq> subst_vars (\<Gamma>(x \<mapsto> untypeify t\<^sub>1)) \<and> valid_ty_subst s \<and> idempotent s" by metis
+    partial_solidify (insert ?v vs) (hsubst s (hsubst [?v \<mapsto> untypeify t\<^sub>1] e'')) = liquify e \<and> 
+    partial_typeify (insert ?v vs) (subst s (subst [?v \<mapsto> untypeify t\<^sub>1] t')) = untypeify t\<^sub>2 \<and>
+    s unifies\<^sub>\<kappa> partial_typeify_constr (insert ?v vs) (constr_subst ?v (untypeify t\<^sub>1) con') \<and> 
+    dom s = vs'' - insert ?v vs \<and> subst_vars s = {} \<and> valid_ty_subst s \<and> idempotent s" by meson
   from tcn_lam have "subst_vars (\<Gamma>(x \<mapsto> untypeify t\<^sub>1)) \<subseteq> vs" by simp
-  moreover from tcn_lam have "?v \<notin> vs" by simp
+  moreover from tcn_lam have FV: "?v \<notin> vs" by simp
   ultimately have "?v \<notin> subst_vars (\<Gamma>(x \<mapsto> untypeify t\<^sub>1))" by blast
-  with tcn_lam TC have "?v \<notin> constr_vars (constr_subst ?v (untypeify t\<^sub>1) con')" by simp
-  with E S have A: "solidify (hsubst (extend_subst ?v (untypeify t\<^sub>1) s) e') = Lam\<^sub>s x t\<^sub>1 e" by simp
-  from S have U: "?v \<notin> dom s" by auto
-  from S have "subst_vars s \<subseteq> subst_vars (\<Gamma>(x \<mapsto> untypeify t\<^sub>1))" by simp
-  moreover from tcn_lam have "subst_vars (\<Gamma>(x \<mapsto> untypeify t\<^sub>1)) \<subseteq> vs \<and> finite vs" by simp
-  ultimately have "?v \<notin> subst_vars s" by fastforce
-  with S U have B: "idempotent (extend_subst ?v (untypeify t\<^sub>1) s)" by simp
-  from S E have C: "extend_subst ?v (untypeify t\<^sub>1) s unifies\<^sub>\<kappa> con" by simp
+  with tcn_lam TC have VCS: "?v \<notin> constr_vars (constr_subst ?v (untypeify t\<^sub>1) con')" by simp
+  have "htvars (hsubst [?v \<mapsto> untypeify t\<^sub>1] e') \<subseteq> 
+    htvars e' - dom [?v \<mapsto> untypeify t\<^sub>1] \<union> subst_vars [?v \<mapsto> untypeify t\<^sub>1]" 
+      by (metis htvars_hsubst)
+  hence "htvars (hsubst [?v \<mapsto> untypeify t\<^sub>1] e') \<subseteq> htvars e' - {?v}" by simp
+  moreover have "htvars (hsubst s (hsubst [?v \<mapsto> untypeify t\<^sub>1] e')) \<subseteq> 
+    htvars (hsubst [?v \<mapsto> untypeify t\<^sub>1] e') - dom s \<union> subst_vars s" by simp
+  ultimately have "htvars (hsubst s (hsubst [?v \<mapsto> untypeify t\<^sub>1] e')) \<subseteq> 
+    htvars e' - {?v} - dom s \<union> subst_vars s" by blast
+  with S have "?v \<notin> htvars (hsubst (extend_subst ?v (untypeify t\<^sub>1) s) e')" by auto
+  with E S VCS have A: "partial_solidify vs (hsubst (extend_subst ?v (untypeify t\<^sub>1) s) e') = 
+    liquify (Lam\<^sub>s x t\<^sub>1 e)" by simp
+  from tcn_lam S have U: "?v \<notin> dom s" by auto
+  with S have B: "idempotent (extend_subst ?v (untypeify t\<^sub>1) s)" by simp
+  from S E FV have "s unifies\<^sub>\<kappa> constr_subst ?v (untypeify t\<^sub>1) (partial_typeify_constr vs con)" 
+    by simp
+  hence C: "extend_subst ?v (untypeify t\<^sub>1) s unifies\<^sub>\<kappa> partial_typeify_constr vs con" by simp
   from E TC have "insert ?v vs \<subseteq> vs'" by (metis vars_expand)
   with tcn_lam have "insert ?v (vs' - insert ?v vs) = vs' - vs" by auto
   with S E have D: "dom (extend_subst ?v (untypeify t\<^sub>1) s) = vs' - vs" by simp
   have VS: "uvars (subst s (untypeify t\<^sub>1)) \<subseteq> uvars (untypeify t\<^sub>1) - dom s \<union> subst_vars s" 
-    by (metis vars_subst)
-  from S have "subst_vars s \<subseteq> subst_vars (\<Gamma>(x := None))" by auto
-  hence "subst_vars s \<subseteq> subst_vars \<Gamma>" by auto
-  with U VS have F: "subst_vars (extend_subst ?v (untypeify t\<^sub>1) s) \<subseteq> subst_vars \<Gamma>" by auto
-  from S E have G: "typeify (subst (extend_subst ?v (untypeify t\<^sub>1) s) tt) = Arrow t\<^sub>1 t\<^sub>2" 
-    by (simp add: expand_extend_subst)
+    by (metis uvars_subst)
+  from S U VS have F: "subst_vars (extend_subst ?v (untypeify t\<^sub>1) s) = {}" by auto
+  from S have AR: "partial_typeify (insert ?v vs) 
+    (subst (map_option (subst [fresh vs \<mapsto> untypeify t\<^sub>1]) \<circ> s) 
+    (subst [fresh vs \<mapsto> untypeify t\<^sub>1] t')) = untypeify t\<^sub>2" by (metis subst_absorb_no_ran)
+  from U have SV: "s ?v = None" by auto
+  have "uvars (subst (extend_subst ?v (untypeify t\<^sub>1) s) t') \<subseteq> 
+    uvars t' - dom (extend_subst ?v (untypeify t\<^sub>1) s) \<union> 
+      subst_vars (extend_subst ?v (untypeify t\<^sub>1) s)" by (metis uvars_subst)
+  with U have "uvars (subst (extend_subst ?v (untypeify t\<^sub>1) s) t') \<subseteq> 
+    uvars t' - insert ?v (dom s) \<union> uvars (subst s (untypeify t\<^sub>1)) \<union> subst_vars s" by simp
+  moreover from S have "?v \<notin> 
+    uvars t' - insert ?v (dom s) \<union> uvars (subst s (untypeify t\<^sub>1)) \<union> subst_vars s" by simp
+  ultimately have "?v \<notin> uvars (subst (extend_subst ?v (untypeify t\<^sub>1) s) t')" by auto
+  with E have "?v \<notin> uvars (subst (extend_subst ?v (untypeify t\<^sub>1) s) tt)" by simp
+  with S E AR SV have G: "partial_typeify vs (subst (extend_subst ?v (untypeify t\<^sub>1) s) tt) = 
+    untypeify (Arrow t\<^sub>1 t\<^sub>2)" by (simp add: expand_extend_subst)
   from S have "valid_ty_subst (extend_subst ?v (untypeify t\<^sub>1) s)" by simp
   with A B C D F G show ?case by blast
 next
@@ -381,25 +438,24 @@ next
   with tcn_app TC1 have E: "e' = App\<^sub>s e\<^sub>1' e\<^sub>2' \<and> tt = Var ?v \<and> vs''' = vs' \<and> 
     con = con\<^sub>1 @ con\<^sub>2 @ [(t\<^sub>1', Ctor ''Arrow'' [t\<^sub>2', Var ?v])]" by (auto simp add: Let_def)
   from tcn_app have "subst_vars \<Gamma> \<subseteq> insert ?v vs" by auto
-  with tcn_app TC1 obtain s\<^sub>1 where S1: "solidify (hsubst s\<^sub>1 e\<^sub>1') = e\<^sub>1 \<and> 
-    typeify (subst s\<^sub>1 t\<^sub>1') = Arrow t\<^sub>1 t\<^sub>2 \<and> dom s\<^sub>1 = vs'' - insert ?v vs \<and> 
-    subst_vars s\<^sub>1 \<subseteq> subst_vars \<Gamma> \<and> s\<^sub>1 unifies\<^sub>\<kappa> con\<^sub>1 \<and> valid_ty_subst s\<^sub>1 \<and> idempotent s\<^sub>1" by fastforce
+  with tcn_app TC1 obtain s\<^sub>1 where S1: "
+    partial_solidify (insert ?v vs) (hsubst s\<^sub>1 e\<^sub>1') = liquify e\<^sub>1 \<and> 
+    partial_typeify (insert ?v vs) (subst s\<^sub>1 t\<^sub>1') = untypeify (Arrow t\<^sub>1 t\<^sub>2) \<and> 
+    dom s\<^sub>1 = vs'' - insert ?v vs \<and> subst_vars s\<^sub>1 = {} \<and> 
+    s\<^sub>1 unifies\<^sub>\<kappa> partial_typeify_constr (insert ?v vs) con\<^sub>1 \<and> valid_ty_subst s\<^sub>1 \<and> idempotent s\<^sub>1" 
+      by fastforce
   from TC1 have V1: "insert ?v vs \<subseteq> vs''" by (metis vars_expand)
   from TC2 E have V2: "vs'' \<subseteq> vs'" by (metis vars_expand)
   with tcn_app V1 have Y: "subst_vars \<Gamma> \<subseteq> vs''" by auto
-  with tcn_app TC1 TC2 Y obtain s\<^sub>2 where S2: "solidify (hsubst s\<^sub>2 e\<^sub>2') = e\<^sub>2 \<and> 
-    typeify (subst s\<^sub>2 t\<^sub>2') = t\<^sub>1 \<and> dom s\<^sub>2 = vs''' - vs'' \<and> subst_vars s\<^sub>2 \<subseteq> subst_vars \<Gamma> \<and> 
-    s\<^sub>2 unifies\<^sub>\<kappa> con\<^sub>2 \<and> valid_ty_subst s\<^sub>2 \<and> idempotent s\<^sub>2" by fastforce
+  with tcn_app TC1 TC2 Y obtain s\<^sub>2 where S2: "partial_solidify vs'' (hsubst s\<^sub>2 e\<^sub>2') = liquify e\<^sub>2 \<and> 
+    partial_typeify vs'' (subst s\<^sub>2 t\<^sub>2') = untypeify t\<^sub>1 \<and> dom s\<^sub>2 = vs''' - vs'' \<and> subst_vars s\<^sub>2 = {} \<and> 
+    s\<^sub>2 unifies\<^sub>\<kappa> partial_typeify_constr vs'' con\<^sub>2 \<and> valid_ty_subst s\<^sub>2 \<and> idempotent s\<^sub>2" by fastforce
   from tcn_app have FV: "?v \<notin> vs" by simp
-  from tcn_app S1 S2 have SV: "subst_vars s\<^sub>1 \<subseteq> vs \<union> subst_vars \<Gamma> \<and> 
-    subst_vars s\<^sub>2 \<subseteq> vs \<union> subst_vars \<Gamma>" by auto
-  with tcn_app have SV: "subst_vars s\<^sub>1 \<subseteq> vs \<and> subst_vars s\<^sub>2 \<subseteq> vs" by auto
   from S1 S2 have DSS: "dom s\<^sub>1 \<inter> dom s\<^sub>2 = {}" by auto
   from tcn_app TC1 S1 have "valid_ty_uexpr t\<^sub>1' \<and> valid_ty_subst s\<^sub>1" by auto
   hence VTS1: "valid_ty_uexpr (subst s\<^sub>1 t\<^sub>1')" by simp
   from tcn_app TC2 S2 have "valid_ty_uexpr t\<^sub>2' \<and> valid_ty_subst s\<^sub>2" by auto
   hence VTS2: "valid_ty_uexpr (subst s\<^sub>2 t\<^sub>2')" by simp
-  hence VUT: "uvars (untypeify t\<^sub>1) \<subseteq> vs \<and> uvars (untypeify t\<^sub>2) \<subseteq> vs" by simp
   let ?s = "extend_subst ?v (untypeify t\<^sub>2) (combine_subst s\<^sub>1 s\<^sub>2)"
   from S1 have D1: "dom s\<^sub>1 = vs'' - insert ?v vs" by simp
   from S2 E have D2: "dom s\<^sub>2 = vs' - vs''" by simp
@@ -412,46 +468,59 @@ next
   with D2 have HV: "dom s\<^sub>2 \<inter> htvars e\<^sub>1' = {}" by auto
   from tcn_app E TC1 TC2 have HV2: "htvars e\<^sub>2' \<subseteq> vs' - vs''" by simp
   have "htvars (hsubst s\<^sub>2 e\<^sub>2') \<subseteq> htvars e\<^sub>2' - dom s\<^sub>2 \<union> subst_vars s\<^sub>2" by simp
-  with D2 SV HV2 have "htvars (hsubst s\<^sub>2 e\<^sub>2') \<subseteq> vs" by auto
-  with D1 SV have "dom s\<^sub>1 \<inter> htvars (hsubst s\<^sub>2 e\<^sub>2') = {}" by auto
-  with S1 S2 VE1 VE2 HV have "solidify (hsubst ?s e\<^sub>1') = e\<^sub>1 \<and> solidify (hsubst ?s e\<^sub>2') = e\<^sub>2" 
-    by simp
-  hence B: "solidify (hsubst ?s (App\<^sub>s e\<^sub>1' e\<^sub>2')) = App\<^sub>s e\<^sub>1 e\<^sub>2" by simp
-  have C: "typeify (subst ?s (Var ?v)) = t\<^sub>2" by simp
-  from S1 S2 have "subst_vars s\<^sub>1 \<subseteq> subst_vars \<Gamma> \<and> subst_vars s\<^sub>2 - dom s\<^sub>1 \<subseteq> subst_vars \<Gamma>" by blast
-  with DSS D3 have D: "subst_vars ?s \<subseteq> subst_vars \<Gamma>" by auto
-  from FV SV have VCS: "?v \<notin> subst_vars s\<^sub>1 \<and> ?v \<notin> subst_vars s\<^sub>2" by auto
-  from D2 SV V1 have D2S1: "dom s\<^sub>2 \<inter> subst_vars s\<^sub>1 = {}" by auto
-  with S1 DSS D3 VCS have UC1: "?s unifies\<^sub>\<kappa> con\<^sub>1" by simp
-  from S2 D3 VCS DSS have UC2: "?s unifies\<^sub>\<kappa> con\<^sub>2" by simp
-  from S1 S2 have "typeify (subst s\<^sub>1 t\<^sub>1') = Arrow (typeify (subst s\<^sub>2 t\<^sub>2')) t\<^sub>2" by simp
-  with VTS1 obtain \<tau>\<^sub>1 \<tau>\<^sub>2 where UT: "subst s\<^sub>1 t\<^sub>1' = Ctor ''Arrow'' [\<tau>\<^sub>1, \<tau>\<^sub>2] \<and> 
-    typeify \<tau>\<^sub>1 = typeify (subst s\<^sub>2 t\<^sub>2') \<and> typeify \<tau>\<^sub>2 = t\<^sub>2" by auto
-
-
-  hence "(\<exists>x. t\<^sub>1' = Var x \<and> s\<^sub>1 x = Some (Ctor ''Arrow'' [\<tau>\<^sub>1, \<tau>\<^sub>2])) \<or> 
-    (\<exists>\<tau>s. t\<^sub>1' = Ctor ''Arrow'' \<tau>s \<and> map (subst s\<^sub>1) \<tau>s = [\<tau>\<^sub>1, \<tau>\<^sub>2])" by auto
-
-
-
-
+  with D2 S2 HV2 have HVS2: "htvars (hsubst s\<^sub>2 e\<^sub>2') = {}" by auto
+  have "htvars (hsubst s\<^sub>1 e\<^sub>1') \<subseteq> htvars e\<^sub>1' - dom s\<^sub>1 \<union> subst_vars s\<^sub>1" by simp
+  with VE1 S1 have "?v \<notin> htvars (hsubst s\<^sub>1 e\<^sub>1')" by blast
+  with S1 S2 VE1 VE2 HV HVS2 have "partial_solidify vs (hsubst ?s e\<^sub>1') = liquify e\<^sub>1 \<and>
+    partial_solidify vs (hsubst ?s e\<^sub>2') = liquify e\<^sub>2" by simp
+  hence B: "partial_solidify vs (hsubst ?s (App\<^sub>s e\<^sub>1' e\<^sub>2')) = liquify (App\<^sub>s e\<^sub>1 e\<^sub>2)" by simp
+  have C: "partial_typeify vs (subst ?s (Var ?v)) = untypeify t\<^sub>2" by simp
+  from S1 S2 DSS D3 have D: "subst_vars ?s = {}" by auto
+  from S1 S2 have VCS: "?v \<notin> subst_vars s\<^sub>1 \<and> ?v \<notin> subst_vars s\<^sub>2" by auto
+  from D2 S1 V1 have D2S1: "dom s\<^sub>2 \<inter> subst_vars s\<^sub>1 = {}" by auto
+  from tcn_app TC1 VG have "?v \<notin> constr_vars con\<^sub>1" by simp
+  with S1 S2 DSS D3 D2S1 have UC1: "?s unifies\<^sub>\<kappa> partial_typeify_constr vs con\<^sub>1" by simp
+  from V1 V2 have VVS': "vs \<subseteq> vs''" by simp
+  from tcn_app TC1 TC2 E have "constr_vars con\<^sub>2 \<subseteq> vs' - vs'' \<union> subst_vars \<Gamma>" by simp
+  with tcn_app have "constr_vars con\<^sub>2 \<inter> vs'' \<subseteq> vs" by auto
+  with S2 VVS' have "s\<^sub>2 unifies\<^sub>\<kappa> partial_typeify_constr vs con\<^sub>2" 
+    by (metis partial_typeify_constr_reduce_subset)
+  with S1 S2 DSS D3 have UC2: "?s unifies\<^sub>\<kappa> partial_typeify_constr vs con\<^sub>2" by simp
   from tcn_app TC1 have UV1: "uvars t\<^sub>1' \<subseteq> vs'' - insert ?v vs \<union> subst_vars \<Gamma>" by simp
   with VG have VT1: "?v \<notin> uvars t\<^sub>1'" by auto
   from tcn_app D2 V1 UV1 have DU1: "dom s\<^sub>2 \<inter> uvars t\<^sub>1' = {}" by auto
   from tcn_app TC1 TC2 E have UV2: "uvars t\<^sub>2' \<subseteq> vs' - vs'' \<union> subst_vars \<Gamma>" by simp
   with VG V1 have VT2: "?v \<notin> uvars t\<^sub>2'" by auto
+  have "uvars (subst s\<^sub>1 t\<^sub>1') \<subseteq> uvars t\<^sub>1' - dom s\<^sub>1 \<union> subst_vars s\<^sub>1" by simp
+  with S1 D1 UV1 have "uvars (subst s\<^sub>1 t\<^sub>1') \<subseteq> 
+    (vs'' - insert ?v vs \<union> subst_vars \<Gamma>) - (vs'' - insert ?v vs) \<union> {}" by auto
+  with tcn_app(6) have "uvars (subst s\<^sub>1 t\<^sub>1') \<subseteq> vs'' - insert ?v vs \<union> vs - (vs'' - insert ?v vs)" 
+    by auto
+  hence US1: "uvars (subst s\<^sub>1 t\<^sub>1') \<subseteq> vs" by auto
   have US2: "uvars (subst s\<^sub>2 t\<^sub>2') \<subseteq> uvars t\<^sub>2' - dom s\<^sub>2 \<union> subst_vars s\<^sub>2" by simp
+  with S2 D2 UV2 have "uvars (subst s\<^sub>2 t\<^sub>2') \<subseteq> (vs' - vs'' \<union> subst_vars \<Gamma>) - (vs' - vs'') \<union> {}" 
+    by auto
+  with tcn_app(6) have "uvars (subst s\<^sub>2 t\<^sub>2') \<subseteq> vs' - vs'' \<union> vs - (vs' - vs'')" 
+    by auto
+  hence US2: "uvars (subst s\<^sub>2 t\<^sub>2') \<subseteq> vs" by auto
   have "(vs'' - insert ?v vs) \<inter> ((vs' - vs'' \<union> vs) - (vs' - vs'') \<union> vs) = {}" by auto
   with tcn_app have "(vs'' - insert ?v vs) \<inter> ((vs' - vs'' \<union> subst_vars \<Gamma>) - (vs' - vs'') \<union> vs) = {}" 
     by auto
-  with SV D2 UV2 have "(vs'' - insert ?v vs) \<inter> (uvars t\<^sub>2' - dom s\<^sub>2 \<union> subst_vars s\<^sub>2) = {}" by auto
+  with S2 D2 UV2 have "(vs'' - insert ?v vs) \<inter> (uvars t\<^sub>2' - dom s\<^sub>2 \<union> subst_vars s\<^sub>2) = {}" by auto
   with D1 US2 have DU2: "dom s\<^sub>1 \<inter> uvars (subst s\<^sub>2 t\<^sub>2') = {}" by fast
-
-
-
-  have "\<tau>\<^sub>1 = subst s\<^sub>2 t\<^sub>2' \<and> \<tau>\<^sub>2 = untypeify t\<^sub>2" by simp
-  with UC1 UC2 VT1 VT2 DU1 DU2 UT have F: "
-    ?s unifies\<^sub>\<kappa> con\<^sub>1 @ con\<^sub>2 @ [(t\<^sub>1', Ctor ''Arrow'' [t\<^sub>2', Var ?v])]" 
+  from D1 have DSV1: "dom s\<^sub>1 \<inter> vs = {}" by auto
+  from D2 V1 have DSV2: "dom s\<^sub>2 \<inter> vs = {}" by auto
+  from S1 obtain tt1 tt2 where SS1: "subst s\<^sub>1 t\<^sub>1' = Ctor ''Arrow'' [tt1, tt2] \<and> 
+    partial_typeify (insert ?v vs) tt1 = untypeify t\<^sub>1 \<and> 
+    partial_typeify (insert ?v vs) tt2 = untypeify t\<^sub>2" by auto
+  from US1 SS1 have "uvars tt1 \<subseteq> vs \<and> uvars tt2 \<subseteq> vs" by simp
+  with FV SS1 have PT1: "partial_typeify vs tt1 = untypeify t\<^sub>1 \<and> 
+    partial_typeify vs tt2 = untypeify t\<^sub>2" by force
+  from US2 have "uvars (subst s\<^sub>2 t\<^sub>2') \<inter> vs'' \<subseteq> vs" by auto
+  with S2 VVS' have "partial_typeify vs (subst s\<^sub>2 t\<^sub>2') = untypeify t\<^sub>1"
+    by (metis partial_typeify_reduce_subset)
+  with FV UC1 UC2 S1 S2 DSV1 DSV2 VT1 VT2 DU1 DU2 SS1 PT1 have F: "
+    ?s unifies\<^sub>\<kappa> partial_typeify_constr vs (con\<^sub>1 @ con\<^sub>2 @ [(t\<^sub>1', Ctor ''Arrow'' [t\<^sub>2', Var ?v])])" 
       by (simp add: expand_extend_subst)
   from DSS VCS V1 D1 D2 S1 S2 D2S1 have G: "idempotent ?s" by simp
   from S1 S2 have "valid_ty_subst ?s" by simp
@@ -469,10 +538,11 @@ proof
     e = erase e\<^sub>t" by fastforce
   have Z: "subst_vars Map.empty \<subseteq> {}" by simp
   have "valid_ty_subst Map.empty \<and> finite {}" by simp
-  with X Y Z have "\<exists>s. solidify (hsubst s e') = e\<^sub>t \<and> typeify (subst s tt) = t \<and> dom s = vs' - {} \<and> 
-    subst_vars s \<subseteq> subst_vars Map.empty \<and> s unifies\<^sub>\<kappa> con \<and> valid_ty_subst s \<and> 
-      idempotent s" using typecheck_fails' by blast
-  then obtain s where "s unifies\<^sub>\<kappa> con \<and> idempotent s" by blast
+  with X Y Z have "\<exists>s. partial_solidify {} (hsubst s e') = liquify e\<^sub>t \<and> 
+    partial_typeify {} (subst s tt) = untypeify t \<and> dom s = vs' - {} \<and> subst_vars s = {} \<and> 
+    s unifies\<^sub>\<kappa> partial_typeify_constr {} con \<and> valid_ty_subst s \<and> idempotent s" 
+    using typecheck_fails' by blast
+  then obtain s where "s unifies\<^sub>\<kappa> partial_typeify_constr {} con \<and> idempotent s" by blast
   hence "\<exists>s'. unify con = Some s' \<and> s specializes s'" by simp
   with X show "False" by simp
 qed
